proof/invariant-abstract/Interrupt_AI.thy
@@ -264,7 +264,7 @@ lemma cancel_ipc_noreply_interrupt_states:
 lemma send_signal_interrupt_states[wp_unsafe]:
   "\<lbrace>\<lambda>s. P (interrupt_states s) \<and> valid_objs s\<rbrace> send_signal a b \<lbrace>\<lambda>_ s. P (interrupt_states s)\<rbrace>"
   apply (simp add: send_signal_def)
-  apply (rule hoare_seq_ext [OF _ get_ntfn_sp])
+  apply (rule hoare_seq_ext [OF _ get_simple_ko_sp])
   apply (rule hoare_pre)
   apply (wp cancel_ipc_noreply_interrupt_states gts_wp hoare_vcg_all_lift thread_get_wp | wpc | simp)+
   apply (clarsimp)
